Syntax.thy
@@ -4,17 +4,6 @@ begin
 
 chapter \<open>While Language Syntax\<close>
 
-type_synonym ('a,'b) basic = "'a set \<times> 'a rel \<times> 'b"
-
-abbreviation vc :: "('a,'b) basic \<Rightarrow> 'a set"
-  where "vc \<alpha> \<equiv> fst \<alpha>"
-
-abbreviation beh :: "('a,'b) basic \<Rightarrow> 'a rel"
-  where "beh \<alpha> \<equiv> fst (snd \<alpha>)"
-
-abbreviation id :: "('a,'b) basic \<Rightarrow> 'b"
-  where "id \<alpha> \<equiv> snd (snd \<alpha>)"
-
 text \<open>
 A While language with non-deterministic choice, iteration and parallel composition.
 Also includes special commands for environment steps, which is useful for describing
@@ -22,7 +11,8 @@ refinement properties. These have no evaluation semantics or rules however.
 \<close>
 datatype ('a,'b) com =
   Nil
-  | Basic "('a,'b) basic"
+  | Basic "'a"
+  | Rel "'b rel"
   | Seq "('a,'b) com" "('a,'b) com" (infixr ";" 80)
   | Choice "('a,'b) com" "('a,'b) com" (infixr "\<sqinter>" 150)
   | Loop "('a,'b) com" ("_*" [100] 150)
@@ -32,12 +22,23 @@ text \<open>Ensure there is no parallelism within a program\<close>
 fun local :: "('a,'b) com \<Rightarrow> bool"
   where 
     "local (c\<^sub>1 || c\<^sub>2) = False" |
+    "local (Rel r) = False" |
     "local (c\<^sub>1 ; c\<^sub>2) = (local c\<^sub>1 \<and> local c\<^sub>2)" |    
     "local (c\<^sub>1 \<sqinter> c\<^sub>2) = (local c\<^sub>1 \<and> local c\<^sub>2)" |  
     "local (c*) = (local c)" |    
     "local _ = True"
 
+text \<open>Identify all operations in a program\<close>
+fun basics :: "('a,'b) com \<Rightarrow> 'a set"
+  where
+    "basics (Basic \<beta>) = {\<beta>}" |
+    "basics (Seq c\<^sub>1 c\<^sub>2) = basics c\<^sub>1 \<union> basics c\<^sub>2" |
+    "basics (Choice c\<^sub>1 c\<^sub>2) = basics c\<^sub>1 \<union> basics c\<^sub>2" |
+    "basics (Parallel c\<^sub>1 c\<^sub>2) = basics c\<^sub>1 \<union> basics c\<^sub>2" |
+    "basics (Loop c) = basics c" |
+    "basics _ = {}"
+
 abbreviation Env
-  where "Env R \<equiv> Basic (UNIV,R\<^sup>*,undefined)"
+  where "Env R \<equiv> Rel (R\<^sup>*)"
 
 end
