ARMv8.thy
@@ -1,0 +1,148 @@
+theory ARMv8
+  imports Syntax
+begin
+
+chapter \<open>ARMv8\<close>
+
+section \<open>State Encoding\<close>
+
+type_synonym ('v,'r,'g) state = "(('g \<Rightarrow> 'v) \<times> ('r \<Rightarrow> 'v))"
+type_synonym ('v,'r,'g) pred = "('v,'r,'g) state \<Rightarrow> bool"
+type_synonym ('v,'r,'g) rpred = "('v,'r,'g) state \<Rightarrow> ('v,'r,'g) state \<Rightarrow> bool"
+
+subsection \<open>Write Operations\<close>
+
+definition pair_upd1 :: "(('a \<Rightarrow> 'b) \<times> ('c \<Rightarrow> 'd)) \<Rightarrow> 'a \<Rightarrow> 'b \<Rightarrow> (('a \<Rightarrow> 'b) \<times> ('c \<Rightarrow> 'd))"
+  where "pair_upd1 f a b = (\<lambda>x. if x = a then b else (fst f) x, snd f)"
+
+definition pair_upd2 :: "(('a \<Rightarrow> 'b) \<times> ('c \<Rightarrow> 'd)) \<Rightarrow> 'c \<Rightarrow> 'd \<Rightarrow> (('a \<Rightarrow> 'b) \<times> ('c \<Rightarrow> 'd))"
+  where "pair_upd2 f a b = (fst f, \<lambda>x. if x = a then b else (snd f) x)"
+
+nonterminal updbinds and updbind
+
+syntax
+  "_updbind1" :: "'a \<Rightarrow> 'a \<Rightarrow> updbind"             ("(2_ :=\<^sub>1/ _)")
+  "_updbind2" :: "'a \<Rightarrow> 'a \<Rightarrow> updbind"             ("(2_ :=\<^sub>2/ _)")
+  ""         :: "updbind \<Rightarrow> updbinds"             ("_")
+  "_updbinds":: "updbind \<Rightarrow> updbinds \<Rightarrow> updbinds" ("_,/ _")
+  "_Update"  :: "'a \<Rightarrow> updbinds \<Rightarrow> 'a"            ("_/'((_)')" [1000, 0] 900)
+
+translations
+  "_Update f (_updbinds b bs)" \<rightleftharpoons> "_Update (_Update f b) bs"
+  "f(x:=\<^sub>1y)" \<rightleftharpoons> "CONST pair_upd1 f x y"
+  "f(x:=\<^sub>2y)" \<rightleftharpoons> "CONST pair_upd2 f x y"
+
+subsection \<open>Read Operations\<close>
+
+abbreviation rg
+  where "rg r m \<equiv> (snd m) r"
+
+abbreviation ld
+  where "ld x m \<equiv> (fst m) x"
+
+section \<open>Instruction Language Definition\<close>
+
+text \<open>Capture a simple set of instructions, covering memory operations and fences\<close>
+(* TODO: Need support for CAS and other RMW *)
+datatype ('v,'r,'g) inst =
+    Load 'r 'g
+  | Store 'g 'r
+  | Op 'r "'v \<Rightarrow> 'v \<Rightarrow> 'v" 'r 'r
+  | Cond "'v \<Rightarrow> bool" 'r
+  | Fence
+  | CFence
+  | StFence
+
+text \<open>Shorthand for a negative condition\<close>
+abbreviation NCond
+  where "NCond f r \<equiv> Cond (\<lambda>v. \<not> f v) r"
+
+text \<open>Instruction Behaviour\<close>
+fun beh\<^sub>i :: "('v,'r,'g) inst \<Rightarrow> ('v,'r,'g) state rel"
+  where
+    "beh\<^sub>i (Store x r) = {(m,m'). m' = m (x :=\<^sub>1 rg r m)}" |
+    "beh\<^sub>i (Load r y) = {(m,m'). m' = m (r :=\<^sub>2 ld y m)}" |
+    "beh\<^sub>i (Op r\<^sub>t f r\<^sub>1 r\<^sub>2) = {(m,m'). m' = m (r\<^sub>t :=\<^sub>2 f (rg r\<^sub>1 m) (rg r\<^sub>2 m))}" |
+    "beh\<^sub>i (Cond f r) = {(m,m'). m = m' \<and> f (rg r m)}" |
+    "beh\<^sub>i _ = Id"
+
+subsection \<open>Reordering\<close>
+
+text \<open>Define forwarding as the elimination of loads given a store to the same address\<close>
+fun fwd :: "('v,'r,'g) inst \<Rightarrow> ('v,'r,'g) inst \<Rightarrow> ('v,'r,'g) inst" 
+  ("_\<langle>_\<rangle>" [1000,0] 1000)
+  where 
+    "fwd (Load r\<^sub>2 y) (Store x r\<^sub>1) = (if (x = y) then Op r\<^sub>2 (\<lambda>x y. x) r\<^sub>1 r\<^sub>1 else Load r\<^sub>2 y)" |
+    "fwd \<alpha> _ = \<alpha>"
+
+text \<open>Define reordering based on Colvin & Smith\<close>
+fun re :: "('v,'r,'g) inst \<Rightarrow> ('v,'r,'g) inst \<Rightarrow> bool" 
+  (infix "\<hookleftarrow>" 100)
+  where
+    "re _ Fence = False" |
+    "re Fence _ = False" |
+    "re (Store _ _) StFence = False" |
+    "re StFence (Store _ _) = False" | 
+    "re (Cond _ _) CFence = False" |
+    "re CFence (Load _ _) = False" |
+    "re (Cond _ _) (Store _ _) = False" |
+    "re (Cond _ r\<^sub>c) (Op r\<^sub>t _ r\<^sub>1 r\<^sub>2) = (r\<^sub>c \<noteq> r\<^sub>t)" |
+    "re (Cond _ r\<^sub>c) (Load r\<^sub>t _) = (r\<^sub>c \<noteq> r\<^sub>t)" |
+    "re (Store y r\<^sub>s) (Load r\<^sub>t x) = (r\<^sub>s \<noteq> r\<^sub>t \<and> x \<noteq> y)" |
+    "re (Store y _) (Store x _) = (x \<noteq> y)" |
+    "re (Store _ r\<^sub>s) (Op r\<^sub>t _ r\<^sub>1 r\<^sub>2) = (r\<^sub>s \<noteq> r\<^sub>t)" |
+    "re (Load r\<^sub>t y) (Load r\<^sub>t' x) = (r\<^sub>t \<noteq> r\<^sub>t' \<and> x \<noteq> y)" |
+    "re (Load r\<^sub>t y) (Store x r\<^sub>s) = (r\<^sub>s \<noteq> r\<^sub>t \<and> x \<noteq> y)" |
+    "re (Load r\<^sub>t _) (Op r\<^sub>t' _ r\<^sub>1 r\<^sub>2) = (r\<^sub>t \<noteq> r\<^sub>t' \<and> r\<^sub>t \<noteq> r\<^sub>1 \<and> r\<^sub>t \<noteq> r\<^sub>2)" |
+    "re (Load r\<^sub>t _) (Cond _ r\<^sub>s) = (r\<^sub>t \<noteq> r\<^sub>s)" |
+    "re (Op r\<^sub>t _ r\<^sub>1 r\<^sub>2) (Load r\<^sub>t' _) = (r\<^sub>t' \<noteq> r\<^sub>t \<and> r\<^sub>t' \<noteq> r\<^sub>1 \<and> r\<^sub>t' \<noteq> r\<^sub>2)" |
+    "re (Op r\<^sub>t _ r\<^sub>1 r\<^sub>2) (Store _ r\<^sub>s) = (r\<^sub>t \<noteq> r\<^sub>s)" |
+    "re (Op r\<^sub>t _ r\<^sub>1 r\<^sub>2) (Op r\<^sub>t' _ r\<^sub>1' r\<^sub>2') = (r\<^sub>t' \<noteq> r\<^sub>t \<and> r\<^sub>t' \<noteq> r\<^sub>1 \<and> r\<^sub>t' \<noteq> r\<^sub>2 \<and> r\<^sub>t \<noteq> r\<^sub>1' \<and> r\<^sub>t \<noteq> r\<^sub>2')" |
+    "re (Op r\<^sub>t _ r\<^sub>1 r\<^sub>2) (Cond _ r\<^sub>s) = (r\<^sub>t \<noteq> r\<^sub>s)" |
+    "re _ _ = True"
+
+section \<open>Instruction Specification Language Definition\<close>
+
+text \<open>Wrap instructions in more abstract specification to facilitate verification\<close>
+type_synonym ('v,'r,'g) ispec = "(('v,'r,'g) pred\<times>('v,'r,'g) inst)"
+
+text \<open>Duplicate forwarding and reordering behaviour of underlying instruction\<close>
+(* TODO: We should provide a method to introduce new VCs for forwarded instructions *)
+fun fwd\<^sub>s :: "('v,'r,'g) ispec \<Rightarrow> ('v,'r,'g) ispec \<Rightarrow> ('v,'r,'g) ispec" 
+  where "fwd\<^sub>s (p,\<alpha>) (_,\<beta>) = (p,fwd \<alpha> \<beta>)" 
+
+fun re\<^sub>s :: "('v,'r,'g) ispec \<Rightarrow> ('v,'r,'g) ispec \<Rightarrow> bool" 
+  where "re\<^sub>s (_,\<alpha>) (_,\<beta>) = re \<alpha> \<beta>" 
+
+fun beh\<^sub>s :: "('v,'r,'g) ispec \<Rightarrow> ('v,'r,'g) state rel" 
+  where "beh\<^sub>s (p,\<alpha>) = beh\<^sub>i \<alpha>" 
+
+fun vc\<^sub>s :: "('v,'r,'g) ispec \<Rightarrow> ('v,'r,'g) state set" 
+  where "vc\<^sub>s (p,\<alpha>) = Collect p" 
+
+text \<open>Common case of a true verification condition\<close>
+abbreviation VC\<^sub>T
+  where "VC\<^sub>T \<alpha> \<equiv> (\<lambda>m. True,\<alpha>)"
+
+section \<open>While Language Definition\<close>
+
+datatype ('v,'r,'g) lang =
+    Skip
+  | Inst "('v,'r,'g) ispec"
+  | Seq "('v,'r,'g) lang" "('v,'r,'g) lang"
+  | If "'v \<Rightarrow> bool" 'r "('v,'r,'g) lang" "('v,'r,'g) lang"
+  | While "'v \<Rightarrow> bool" 'r "('v,'r,'g) pred" "('v,'r,'g) lang"
+
+text \<open>Convert the While language into the com language expected by the underlying logic\<close> 
+(* TODO: This should be later, closer to the soundness proof *)
+fun lift\<^sub>c :: "('v,'r,'g) lang \<Rightarrow> (('v,'r,'g) ispec,('v,'r,'g) state) com"
+  where
+    "lift\<^sub>c Skip = com.Nil" |
+    "lift\<^sub>c (Inst \<alpha>) = Basic \<alpha>"|
+    "lift\<^sub>c (Seq c\<^sub>1 c\<^sub>2) = (com.Seq (lift\<^sub>c c\<^sub>1) (lift\<^sub>c c\<^sub>2))" |
+    "lift\<^sub>c (If f r c\<^sub>1 c\<^sub>2) = (Choice (com.Seq (Basic (VC\<^sub>T (Cond f r))) (lift\<^sub>c c\<^sub>1)) 
+                                    (com.Seq (Basic (VC\<^sub>T (NCond f r))) (lift\<^sub>c c\<^sub>2)))" |
+    "lift\<^sub>c (While f r I c) = (com.Seq ((com.Seq (Basic (VC\<^sub>T (Cond f r))) (lift\<^sub>c c))*) 
+                                      (Basic (VC\<^sub>T (NCond f r))))"
+
+end
