ARMv8_Rules.thy
@@ -1,0 +1,412 @@
+theory ARMv8_Rules
+  imports Refine ARMv8 
+begin
+
+named_theorems pred_defs
+definition conj  (infixr "\<and>\<^sub>p" 35)
+  where "conj l r \<equiv> \<lambda>m. (l m) \<and> (r m)"
+definition entail (infix "\<turnstile>\<^sub>p" 25)
+  where "entail P Q \<equiv> \<forall>m. P m \<longrightarrow> Q m"
+definition assert
+  where "assert b \<equiv> \<lambda>m. b"
+declare assert_def [pred_defs]
+declare entail_def [pred_defs]
+declare conj_def [pred_defs]
+definition stabilize 
+  where "stabilize R P \<equiv> \<lambda>m. \<forall>m'. R m m' \<longrightarrow> P m'"
+definition reflexive 
+  where "reflexive R \<equiv> \<forall>m . R m  m"
+definition transitive 
+  where "transitive R \<equiv> \<forall>m m' m''. R m m' \<longrightarrow> R m' m'' \<longrightarrow> R m m''"
+
+section \<open>Predicate Transformations\<close>
+
+text \<open>Transform a predicate based on an instruction\<close>
+fun wp\<^sub>i :: "('v,'r,'g) inst \<Rightarrow> ('v,'r,'g) pred \<Rightarrow> ('v,'r,'g) pred" 
+  where 
+    "wp\<^sub>i (Store x r) Q = (\<lambda>m. Q (m (x :=\<^sub>1 rg r m)))" | 
+    "wp\<^sub>i (Load r x) Q = (\<lambda>m. Q (m (r :=\<^sub>2 ld x m)))" | 
+    "wp\<^sub>i (Op r\<^sub>t f r\<^sub>1 r\<^sub>2) Q = (\<lambda>m. Q (m (r\<^sub>t :=\<^sub>2 f (rg r\<^sub>1 m) (rg r\<^sub>2 m))))" |
+    "wp\<^sub>i (Cond f r) Q = (\<lambda>m. (f (rg r m)) \<longrightarrow> Q m)" | 
+    "wp\<^sub>i _ Q = Q"
+
+fun wp\<^sub>s  :: "('v,'r,'g) ispec \<Rightarrow> ('v,'r,'g) pred \<Rightarrow> ('v,'r,'g) pred"
+  where
+    "wp\<^sub>s (p,\<alpha>) Q = (p \<and>\<^sub>p wp\<^sub>i \<alpha> Q)"
+
+text \<open>The WP predicate transformer given a rely R and guarantee G\<close>
+fun wp :: "('v,'r,'g) rpred \<Rightarrow> ('v,'r,'g) rpred \<Rightarrow> ('v,'r,'g) lang \<Rightarrow> ('v,'r,'g) pred \<Rightarrow> ('v,'r,'g) pred"
+  where
+    "wp R G Skip Q = Q" |
+    "wp R G (Inst \<alpha>) Q = stabilize R (wp\<^sub>s \<alpha> Q)" |
+    "wp R G (Seq c\<^sub>1 c\<^sub>2) Q = wp R G c\<^sub>1 (wp R G c\<^sub>2 Q)" |
+    "wp R G (If f r c\<^sub>1 c\<^sub>2) Q = stabilize R (wp\<^sub>i (Cond f r) (wp R G c\<^sub>1 Q) \<and>\<^sub>p 
+                                           wp\<^sub>i (NCond f r) (wp R G c\<^sub>2 Q))" |
+    "wp R G (While f r I c) Q = (stabilize R I \<and>\<^sub>p
+                                (assert (I \<turnstile>\<^sub>p (wp\<^sub>i (Cond f r) (wp R G c (stabilize R I))) \<and>\<^sub>p 
+                                              wp\<^sub>i (NCond f r) Q)))"
+
+text \<open>Convert a state predicate into the shallow-embedding\<close>
+definition state
+  where "state P \<equiv> {(m). P m}"
+
+text \<open>Convert a state relation into the shallow-embedding\<close>
+definition step
+  where "step P \<equiv> {((m),(m')). P m m'}"
+
+section \<open>Wellformedness\<close>
+
+text \<open>Couple all wellformedness conditions into a single definition\<close>
+definition wellformed :: "('v,'r,'g) rpred \<Rightarrow> ('v,'r,'g) rpred \<Rightarrow> ('v,'r,'g) pred \<Rightarrow> bool"
+  where "wellformed R G Q \<equiv> 
+    stable (step R) (state Q)  \<and> reflexive R \<and> transitive R \<and> reflexive G" 
+
+lemma G_refl [intro]:
+  assumes wf: "wellformed R G Q"
+  shows "G m m" 
+  using wf unfolding wellformed_def reflexive_def by blast
+
+text \<open>Establish wellformedness of a false predicate\<close>
+lemma wf_false:
+  "\<forall>m. \<not> P m \<Longrightarrow> wellformed R G Q \<Longrightarrow> wellformed R G P"
+  unfolding wellformed_def stable_def by (auto simp: state_def)
+
+text \<open>Show that a stabilized predicate is stable\<close>
+lemma stabilize_stable [intro]:
+  assumes wf: "wellformed R G P"
+  shows "stable (step R) (state (stabilize R Q))"
+  unfolding stable_def state_def step_def
+proof (clarsimp)
+  fix m m'
+  assume a: "(stabilize R Q) m" "R m m'"
+  have "\<forall>m''. R m' m'' \<longrightarrow> R m m''"
+    using assms a(2) unfolding wellformed_def transitive_def by blast
+  thus "(stabilize R Q) m'" using a(1) by (auto simp: stabilize_def)
+qed
+
+text \<open>Stabilization preserves wellformedness\<close>
+lemma stabilize_wellformed [intro]:
+  assumes "wellformed R G P"
+  shows "wellformed R G (stabilize R Q)" (is "wellformed R G ?P")
+proof -
+  have "stable (step R) (state ?P)" 
+    using stabilize_stable assms by blast
+  thus ?thesis using assms unfolding wellformed_def by blast
+qed
+
+text \<open>WP preserves wellformedness\<close>
+lemma wellformed_actI [intro]:
+  assumes "wellformed R G Q"
+  shows "wellformed R G (wp R G (Inst \<alpha>) Q)"
+  using assms wellformed_def by auto
+
+text \<open>Elimination rule to ignore the stabilization process\<close>
+lemma stabilizeE:
+  assumes "stabilize R P m"
+  assumes "wellformed R G Q"
+  obtains "P m"
+  using assms unfolding wellformed_def reflexive_def stabilize_def by blast
+
+section \<open>Program Wellformedness\<close>
+
+text \<open>We require all instructions in a program to conform to the guarantee\<close>
+
+text \<open>Compute the verification condition necessary for an instruction to conform to a guarantee G\<close>
+definition guar\<^sub>i :: "('v,'r,'g) inst \<Rightarrow> ('v,'r,'g) rpred \<Rightarrow> ('v,'r,'g) pred"
+  where "guar\<^sub>i i G \<equiv> \<lambda>m. \<forall>m'. (m,m') \<in> beh\<^sub>i i \<longrightarrow> (G m m' \<or> m = m')"
+
+fun guar\<^sub>s :: "('v,'r,'g) ispec \<Rightarrow> ('v,'r,'g) rpred \<Rightarrow> bool"
+  where "guar\<^sub>s (p,\<alpha>) G = (p \<turnstile>\<^sub>p guar\<^sub>i \<alpha> G)"
+
+text \<open>Ensure all operations have preconditions strong enough to discharge their guarantee\<close>
+fun guar\<^sub>c
+  where
+    "guar\<^sub>c (Inst \<alpha>) G = guar\<^sub>s \<alpha> G" |
+    "guar\<^sub>c (Seq c\<^sub>1 c\<^sub>2) G = (guar\<^sub>c c\<^sub>1 G \<and> guar\<^sub>c c\<^sub>2 G)" |
+    "guar\<^sub>c (If f v c\<^sub>1 c\<^sub>2) G = (guar\<^sub>c c\<^sub>1 G \<and> guar\<^sub>c c\<^sub>2 G)" |
+    "guar\<^sub>c (While f v I c) G = (guar\<^sub>c c G)" |
+    "guar\<^sub>c _ _ = True"
+
+section \<open>Soundness\<close>
+
+subsection \<open>Interpretation of General Logic\<close>
+
+fun act_ref :: "('v,'r,'g) ispec \<Rightarrow> ('v,'r,'g) ispec \<Rightarrow> bool" 
+  where "act_ref (p,\<alpha>) (q,\<beta>) = (\<alpha> = \<beta> \<and> (p \<turnstile>\<^sub>p q))"
+
+interpretation refine vc\<^sub>s beh\<^sub>s fwd\<^sub>s re\<^sub>s act_ref
+  by (unfold_locales) (auto simp: pred_defs)
+
+abbreviation lrules_abv ("_,_ \<turnstile>\<^sub>l _ {_} _" [20,0,0,0,20] 20)
+  where "lrules_abv \<equiv> lrules"
+
+abbreviation rules_abv ("_,_ \<turnstile> _ {_} _" [20,0,0,0,20] 20)
+  where "rules_abv \<equiv> rules"
+
+abbreviation lifted_abv ("_,_ \<turnstile>\<^sub>s _ {_} _" [20,0,0,0,20] 20)
+  where "lifted_abv R G P c Q \<equiv> step R,step G \<turnstile>\<^sub>l state P {lift\<^sub>c c} state Q"
+
+abbreviation validity_abv  ("\<Turnstile> _ SAT [_, _, _, _]" [60,0,0,0,0] 45) 
+  where "validity_abv c P R G Q \<equiv> validity (lift\<^sub>c c) (state P) (step R) (step G) (state Q)"
+
+text \<open>An ordering property on contexts\<close>
+definition context_order 
+  ("_,_ \<turnstile>\<^sub>w _ \<ge> _" [100,0,0,100] 60)
+  where "context_order R G P Q \<equiv> wellformed R G Q \<longrightarrow> ((P \<turnstile>\<^sub>p Q) \<and> wellformed R G P)"
+
+text \<open>The validity property we intend to show, abstracts over the preservation of wellformedness\<close>
+definition valid 
+  ("_,_ \<turnstile>\<^sub>w _ {_} _" [100,0,0,100] 60)
+  where "valid R G P c Q \<equiv> (guar\<^sub>c c G \<and> wellformed R G Q) \<longrightarrow> ((R,G \<turnstile>\<^sub>s P {c} Q) \<and> wellformed R G P)"
+
+subsection \<open>Instruction Soundness\<close>
+
+text \<open>WP correctly transforms the state for an instruction\<close>
+lemma wp_sound [intro]:
+  assumes wf: "wellformed R G Q" 
+  shows "state (stabilize R (wp\<^sub>s \<alpha> Q)) \<subseteq> wp\<^sub>\<alpha> \<alpha> (state Q)"
+  using wf by (cases \<alpha>, rename_tac p i, case_tac i) 
+              (auto simp add: state_def wp_def pred_defs elim!: stabilizeE)
+
+text \<open>The guar check is correct\<close>
+lemma guar_correct [simp]:
+  "guar \<alpha> (step G) = guar\<^sub>c (Inst \<alpha>) G"
+  by (cases \<alpha>) (auto simp: guar\<^sub>i_def pred_defs step_def)
+
+text \<open>WP soundly computes an instructions weakest precondition\<close>
+lemma inst_sound [intro]:
+  assumes "wellformed R G Q" "guar\<^sub>c (Inst \<alpha>) G"
+  shows "R,G \<turnstile>\<^sub>s wp R G (Inst \<alpha>) Q {Inst \<alpha>} Q"
+proof (clarsimp, rule lrules.basic, simp add: atomic_rule_def, intro conjI)
+  show "state (stabilize R (wp\<^sub>s \<alpha> Q)) \<subseteq> wp\<^sub>\<alpha> \<alpha> (state Q)" 
+    using assms(1) wp_sound by blast
+qed (insert assms, auto simp: wellformed_def)
+
+text \<open>Bundle the inst rule with a precondition rewrite\<close>
+lemma inst_conseq [intro]:
+  assumes "wellformed R G Q" "guar\<^sub>c (Inst \<alpha>) G"
+  assumes "P \<turnstile>\<^sub>p wp R G (Inst \<alpha>) Q"
+  shows "step R,step G \<turnstile>\<^sub>l state P {Basic \<alpha>} state Q"
+  using inst_sound[OF assms(1,2)] apply simp
+proof (rule lrules.conseq)
+  show "state P \<subseteq> state (wp R G (Inst \<alpha>) Q)"
+    using assms(3) by (auto simp: entail_def state_def)
+qed auto
+
+subsection \<open>Base Introduction Rules\<close>
+
+text \<open>Reflexive Ordering\<close>
+lemma reflOrd [intro]:
+  "R,G \<turnstile>\<^sub>w P \<ge> P"
+  unfolding context_order_def by (auto simp: pred_defs)
+
+text \<open>Assert Ordering\<close>
+lemma assertOrd:
+  "R,G \<turnstile>\<^sub>w P \<and>\<^sub>p assert A \<ge> P"
+  by (cases A) (auto simp: context_order_def pred_defs intro: wf_false) 
+
+text \<open>Stabilize Ordering\<close>
+lemma stabilizeOrd:
+  assumes "P \<turnstile>\<^sub>p Q" 
+  shows "R,G \<turnstile>\<^sub>w stabilize R P \<ge> Q"
+  using assms stabilizeE unfolding context_order_def entail_def
+  by blast
+
+text \<open>Skip Rule\<close>
+lemma skipWP:
+  "R,G \<turnstile>\<^sub>w Q {Skip} Q"
+  by (auto simp: context_order_def valid_def wellformed_def)
+
+text \<open>Instruction Rule\<close>
+lemma instWP:
+  "R,G \<turnstile>\<^sub>w wp R G (Inst \<alpha>) Q {Inst \<alpha>} Q"
+  unfolding valid_def using inst_sound[of R G Q \<alpha>] by auto
+ 
+text \<open>Sequential Rule\<close>
+lemma seqWP:
+  "R,G \<turnstile>\<^sub>w P {c\<^sub>1} Q \<Longrightarrow> R,G \<turnstile>\<^sub>w M {c\<^sub>2} P \<Longrightarrow> R,G \<turnstile>\<^sub>w M {Seq c\<^sub>2 c\<^sub>1} Q"
+  unfolding valid_def by auto
+
+lemma guar_cond [simp]:
+  "guar\<^sub>i (Cond f r) G = (\<lambda>m. True)"
+  by (auto simp add: pred_defs guar\<^sub>i_def)
+
+lemma [simp]:
+  "(P \<turnstile>\<^sub>p P) = True"
+  by (auto simp add: pred_defs guar\<^sub>i_def)
+
+text \<open>Stabilization preserves entailment\<close>
+lemma stabilize_entail [intro]:
+  assumes "P \<turnstile>\<^sub>p Q"
+  shows "stabilize R P \<turnstile>\<^sub>p stabilize R Q"
+  using assms by (clarsimp simp add: entail_def stabilize_def)
+
+text \<open>If Rule\<close>
+lemma ifWP:
+  assumes "R,G \<turnstile>\<^sub>w P\<^sub>1 {c\<^sub>1} Q"
+  assumes "R,G \<turnstile>\<^sub>w P\<^sub>2 {c\<^sub>2} Q"
+  shows "R,G \<turnstile>\<^sub>w stabilize R (wp\<^sub>i (Cond f r) P\<^sub>1 \<and>\<^sub>p wp\<^sub>i (NCond f r) P\<^sub>2) {If f r c\<^sub>1 c\<^sub>2} Q"
+  using assms 
+  apply (clarsimp simp add: valid_def)
+  apply (intro impI conjI lrules.choice lrules.seq stabilize_wellformed; assumption?)
+  by (intro inst_conseq; simp; intro stabilize_entail; simp add: pred_defs)+
+
+text \<open>While Rule\<close>
+lemma whileWP:
+  assumes "I \<turnstile>\<^sub>p wp\<^sub>i (Cond f r) P \<and>\<^sub>p wp\<^sub>i (NCond f r) Q"
+  assumes "R,G \<turnstile>\<^sub>w P {c} stabilize R I" (is "R,G \<turnstile>\<^sub>w P {c} ?I")
+  shows "R,G \<turnstile>\<^sub>w ?I {While f r I c} Q"
+  unfolding valid_def lift\<^sub>c.simps
+proof (intro impI conjI lrules.choice lrules.seq stabilize_wellformed; assumption?)
+  assume "guar\<^sub>c (While f r I c) G \<and> wellformed R G Q"
+  thus "step R,step G \<turnstile>\<^sub>l (state ?I) {Basic (VC\<^sub>T (NCond f r))} state Q"
+    using assms(1) 
+    by (intro inst_conseq; simp; intro stabilize_entail; simp add: pred_defs)
+next
+  assume "guar\<^sub>c (While f r I c) G \<and> wellformed R G Q"
+  hence "guar\<^sub>c c G" "wellformed R G ?I" by auto
+  thus "step R,step G \<turnstile>\<^sub>l state ?I {(Basic (VC\<^sub>T (Cond f r)) ; lift\<^sub>c c)*} state ?I"
+    using assms
+    apply (intro lrules.loop lrules.seq stabilize_stable; simp add: valid_def)
+    defer 1
+    by blast (intro inst_conseq; simp; intro stabilize_entail; simp add: pred_defs)
+qed auto
+
+lemma local_lift [intro]:
+  "local (lift\<^sub>c c)"
+  by (induct c) auto
+
+lemma guar_all:
+  "guar\<^sub>c c G \<Longrightarrow> \<forall>\<beta>\<in>basics (lift\<^sub>c c). guar \<beta> (step G)"
+  by (induct c) auto
+
+text \<open>False Rule\<close>
+lemma falseWP:
+  assumes "P \<turnstile>\<^sub>p (\<lambda>m. False)"
+  shows "R,G \<turnstile>\<^sub>w P {c} Q"
+  using assms unfolding valid_def
+  apply (intro conjI impI guar_all lrules.conseq[OF falseI, where ?G="step G"])
+  by (auto simp: entail_def state_def intro: wf_false)
+
+text \<open>Precondition Rewrite Rule\<close>
+lemma rewriteWP:
+  "R,G \<turnstile>\<^sub>w P {c} Q \<Longrightarrow> R,G \<turnstile>\<^sub>w M \<ge> P \<Longrightarrow> R,G \<turnstile>\<^sub>w M {c} Q"
+proof (clarsimp simp add: valid_def context_order_def)
+  assume a: "M \<turnstile>\<^sub>p P"
+  assume "R,G \<turnstile>\<^sub>s P {c} Q "
+  thus "R,G \<turnstile>\<^sub>s M {c} Q" by (rule lrules.conseq) (insert a, auto simp: entail_def state_def)
+qed
+
+text \<open>Assert Rule\<close>
+
+lemma assertWP:
+  assumes "A \<longrightarrow> R,G \<turnstile>\<^sub>w P {c} Q"
+  shows "R,G \<turnstile>\<^sub>w (P \<and>\<^sub>p assert A) {c} Q"
+proof (cases A)
+  case True
+  then show ?thesis using assms by (intro rewriteWP[OF _ assertOrd], simp)
+next
+  case False
+  then show ?thesis by (intro falseWP, auto simp: pred_defs)
+qed 
+
+subsection \<open>Rewrite Introduction Rules\<close>
+
+text \<open>Skip Rewrite Rule\<close>
+lemma skipRW:
+  assumes "R,G \<turnstile>\<^sub>w P \<ge> Q" 
+  shows "R,G \<turnstile>\<^sub>w P {Skip} Q"
+  using rewriteWP[OF skipWP assms] .
+
+text \<open>Act Rewrite Rule\<close>
+lemma actRW:
+  assumes "R,G \<turnstile>\<^sub>w P \<ge> wp R G (Inst \<alpha>) Q"
+  shows "R,G \<turnstile>\<^sub>w P {Inst \<alpha>} Q"
+  using rewriteWP[OF instWP assms] .
+
+text \<open>If Rewrite Rule\<close>
+lemma ifRW:
+  assumes "R,G \<turnstile>\<^sub>w P \<ge> stabilize R (wp\<^sub>i (Cond f r) P\<^sub>1 \<and>\<^sub>p wp\<^sub>i (NCond f r) P\<^sub>2)"
+  assumes "R,G \<turnstile>\<^sub>w P\<^sub>1 {c\<^sub>1} Q"
+  assumes "R,G \<turnstile>\<^sub>w P\<^sub>2 {c\<^sub>2} Q"
+  shows "R,G \<turnstile>\<^sub>w P {If f r c\<^sub>1 c\<^sub>2} Q"
+  using rewriteWP[OF ifWP[OF assms(2,3)] assms(1)] . 
+
+text \<open>While Rewrite Rule\<close>
+lemma whileRW:
+  assumes order: "R,G \<turnstile>\<^sub>w N \<ge> stabilize R I"
+  assumes recur: "R,G \<turnstile>\<^sub>w P {c} stabilize R I"
+  assumes side: "I \<turnstile>\<^sub>p wp\<^sub>i (Cond f r) P \<and>\<^sub>p wp\<^sub>i (NCond f r) Q"
+  shows "R,G \<turnstile>\<^sub>w N {While f r I c} Q"
+  using rewriteWP[OF whileWP[OF side recur] order] .
+
+subsection \<open>Soundness\<close>
+
+lemma wp_valid:
+  shows "R,G \<turnstile>\<^sub>w wp R G c Q {c} Q" 
+proof (induct c arbitrary: Q)
+  case Skip
+  thus ?case using skipWP by auto
+next
+  case (Inst \<beta>)
+  thus ?case using instWP by blast
+next
+  case (Seq c\<^sub>1 c\<^sub>2)
+  thus ?case using seqWP unfolding wp.simps by blast
+next
+  case (If f r c\<^sub>1 c\<^sub>2)
+  thus ?case using ifWP unfolding wp.simps by metis
+next
+  case (While f r I c)
+  thus ?case unfolding wp.simps
+    by (intro assertWP impI whileRW) (auto simp add: pred_defs)
+qed
+
+text \<open>Soundness lemma for WP reasoning over ARMv8 with verification conditions\<close>
+theorem armv8_wp_sound_vc:
+  assumes wf: "transitive R" "reflexive R" "reflexive G" 
+  assumes st: "stable (step R) (state Q)" 
+  assumes g: "guar\<^sub>c c G"
+  assumes P: "P \<turnstile>\<^sub>p wp R G c Q"
+  assumes i: "inter (step R) (step G) (lift\<^sub>c c)" (* Rephrase this in terms of the ARMv8 analysis *)
+  shows "\<Turnstile> c SAT [P, R, G, Q]"
+proof -
+  have "wellformed R G Q" using wf st by (auto simp: wellformed_def)
+  hence "R,G \<turnstile>\<^sub>s wp R G c Q {c} Q" using g wp_valid unfolding valid_def by blast
+  hence "R,G \<turnstile>\<^sub>s P {c} Q" by (rule lrules.conseq) (insert P, auto simp: state_def entail_def)
+  thus ?thesis using i by (intro sound thread) auto
+qed
+
+text \<open>Refine via the elimination of verification conditions\<close>
+fun no_vc
+  where 
+    "no_vc Skip = Skip" |
+    "no_vc (Inst (p,\<alpha>)) = Inst (\<lambda>m. True,\<alpha>)" |
+    "no_vc (Seq c\<^sub>1 c\<^sub>2) = Seq (no_vc c\<^sub>1) (no_vc c\<^sub>2)" |
+    "no_vc (If f r c\<^sub>1 c\<^sub>2) = If f r (no_vc c\<^sub>1) (no_vc c\<^sub>2)" |
+    "no_vc (While f r I c) = While f r I (no_vc c)"
+
+text \<open>Prove elimination of verification conditions is a valid refinement\<close>
+lemma no_vc_ref:
+  "lang_ref (lift\<^sub>c c) (lift\<^sub>c (no_vc c))"
+proof (induct c)
+  case (Inst x)
+  then show ?case by (cases x) (auto simp: pred_defs)
+qed auto
+
+text \<open>Soundness lemma for WP reasoning over ARMv8\<close>
+theorem armv8_wp_sound:
+  assumes wf: "transitive R" "reflexive R" "reflexive G" 
+  assumes st: "stable (step R) (state Q)" 
+  assumes g: "guar\<^sub>c c G"
+  assumes P: "P \<turnstile>\<^sub>p wp R G c Q"
+  assumes i: "inter (step R) (step G) (lift\<^sub>c c)" (* Rephrase this in terms of the ARMv8 analysis *)
+  shows "\<Turnstile> (no_vc c) SAT [P, R, G, Q]"
+proof -
+  have "wellformed R G Q" using wf st by (auto simp: wellformed_def)
+  hence "R,G \<turnstile>\<^sub>s wp R G c Q {c} Q" using g wp_valid unfolding valid_def by blast
+  hence "R,G \<turnstile>\<^sub>s P {c} Q" by (rule lrules.conseq) (insert P, auto simp: state_def entail_def)
+  thus ?thesis using i no_vc_ref by (intro refine_sound thread) auto
+qed
+
+end
